src/Lean/Meta/Sym/Simp/Main.lean
@@ -7,6 +7,7 @@ module
 prelude
 public import Lean.Meta.Sym.Simp.SimpM
 import Lean.Meta.Sym.AlphaShareBuilder
+import Lean.Meta.AppBuilder
 import Lean.Meta.Sym.Simp.Result
 import Lean.Meta.Sym.Simp.Simproc
 import Lean.Meta.Sym.Simp.App
@@ -17,12 +18,34 @@ import Lean.Meta.WHNF
 namespace Lean.Meta.Sym.Simp
 open Internal
 
+def reduceLambda : Simproc := fun e => do
+  unless e.isApp do
+    return Result.rfl
+  unless e.getAppFn.isLambda do
+    return Result.rfl
+  let new := e.headBeta
+  return (Result.step new (←mkEqRefl new))
+
 def simpStep : Simproc := fun e => do
   match e with
   | .lit _ | .sort _ | .bvar _ | .const .. | .fvar _  | .mvar _ => return .rfl
-  | .proj .. =>
-    let some e ← reduceProj? e | throwError "could not reduce projection"
-    simp e
+  | .proj typeName idx struct =>
+      let res ← simp struct
+      match res with
+      | .rfl .. =>
+        let some e ← reduceProj? e | return .rfl
+        return .step e (← mkEqRefl e) (done := true)
+      | .step _ proof _ =>
+        if let some e ← reduceProj? e then
+          let res ← simp e
+          return res
+        let fType ← inferType struct
+        let congrArgFun ← withLocalDecl (← mkFreshUserName `x) BinderInfo.default fType fun var => do
+          let theoremLhs := Expr.proj typeName idx var
+          mkLambdaFVars #[var] theoremLhs
+        let congrArg ← mkCongrArg congrArgFun proof
+        let some reduced ← reduceProj? congrArg | return .step congrArg proof (done := true)
+        return .step reduced proof
   | .mdata m b =>
     let r ← simp b
     match r with
@@ -31,7 +54,11 @@ def simpStep : Simproc := fun e => do
   | .lam .. => simpLambda e
   | .forallE .. => simpForall e
   | .letE .. => simpLet e
-  | .app .. => simpAppArgs e
+  | .app .. =>
+      (simpAppArgs >> reduceLambda) e
+
+
+
 
 abbrev cacheResult (e : Expr) (r : Result) : SimpM Result := do
   modify fun s => { s with cache := s.cache.insert { expr := e } r }
@@ -39,6 +66,7 @@ abbrev cacheResult (e : Expr) (r : Result) : SimpM Result := do
 
 @[export lean_sym_simp]
 def simpImpl (e₁ : Expr) : SimpM Result := withIncRecDepth do
+  trace[Meta.Tactic] "Called simp with {e₁}"
   let numSteps := (← get).numSteps
   if numSteps >= (← getConfig).maxSteps then
     throwError "`simp` failed: maximum number of steps exceeded"
@@ -51,11 +79,15 @@ def simpImpl (e₁ : Expr) : SimpM Result := withIncRecDepth do
   let r₁ ← pre e₁
   match r₁ with
   | .rfl true | .step _ _ true => cacheResult e₁ r₁
-  | .step e₂ h₁ false => cacheResult e₁ (← mkEqTransResult e₁ e₂ h₁ (← simp e₂))
+  | .step e₂ h₁ false =>
+    trace[Meta.Tactic] "Obtained {e₂} in pre"
+    cacheResult e₁ (← mkEqTransResult e₁ e₂ h₁ (← simp e₂))
   | .rfl false =>
   let r₂ ← (simpStep >> post) e₁
   match r₂ with
   | .rfl _ | .step _ _ true => cacheResult e₁ r₂
-  | .step e₂ h₁ false => cacheResult e₁ (← mkEqTransResult e₁ e₂ h₁ (← simp e₂))
+  | .step e₂ h₁ false =>
+    trace[Meta.Tactic] "Obtained {e₂} in post"
+    cacheResult e₁ (← mkEqTransResult e₁ e₂ h₁ (← simp e₂))
 
 end Lean.Meta.Sym.Simp
