src/Lean/Meta/Sym/Simp/Rewrite.lean
@@ -13,6 +13,7 @@ public import Lean.Meta.Sym.Simp.Discharger
 import Lean.Meta.Sym.InstantiateS
 import Lean.Meta.Sym.InstantiateMVarsS
 import Lean.Meta.Sym.Simp.DiscrTree
+public import Lean.Meta.AppBuilder
 namespace Lean.Meta.Sym.Simp
 open Grind
 
@@ -55,11 +56,12 @@ public def Theorem.rewrite (thm : Theorem) (e : Expr) (d : Discharger := dischar
             args := args.set i val
           else
             -- **Note**: Failed to discharge hypothesis.
+            trace[Meta.Tactic] "Could not discharge {arg}"
             return .rfl
       else if arg.hasMVar then
         let arg ← instantiateMVarsS arg
         args := args.set i arg
-    let proof := mkValue thm.expr thm.pattern us args.toArray
+    let mut proof := mkValue thm.expr thm.pattern us args.toArray
     let rhs   := thm.rhs.instantiateLevelParams thm.pattern.levelParams us
     let rhs   ← share rhs
     let expr  ← instantiateRevBetaS rhs args.toArray
@@ -69,6 +71,55 @@ public def Theorem.rewrite (thm : Theorem) (e : Expr) (d : Discharger := dischar
       return .step expr proof
   else
     return .rfl
+
+public def Theorem.rewriteMatchCongrThm (thm : Theorem) (e : Expr) (d : Discharger := dischargeNone) (heq := false) : SimpM Result :=
+  /-
+  **Note**: We use `withNewMCtxDepth` to ensure auxiliary metavariables used during the `match?`
+  do not pollute the metavariable context.
+  Thus, we must ensure that all assigned variables have be instantiate.
+  -/
+  withNewMCtxDepth do
+  if let some result ← thm.pattern.match? e then
+    trace[Meta.Tactic] "Successfully matched: {thm.expr}"
+    -- **Note**: Potential optimization: check whether pattern covers all variables.
+    let mut args := result.args.toVector
+    let us ← result.us.mapM instantiateLevelMVars
+    trace[Meta.Tactic] "Args: {args.toArray}"
+    for h : i in *...args.size do
+      let arg := args[i]
+      if let .mvar mvarId := arg then
+        if (← mvarId.isAssigned) then
+          let arg ← instantiateMVarsS arg
+          args := args.set i arg
+        else
+          let decl ← mvarId.getDecl
+          if let some val ← d decl.type then
+            let val ← instantiateMVarsS val
+            mvarId.assign val
+            args := args.set i val
+      else if arg.hasMVar then
+        let arg ← instantiateMVarsS arg
+        args := args.set i arg
+    if (← args.allM fun x => x.mvarId!.isAssigned) then
+      trace[Meta.Tactic] "Unsolved constraints"
+      return .rfl
+    args ← args.mapM fun arg => return ← instantiateMVarsS arg
+    let proof := mkValue thm.expr thm.pattern us args.toArray
+    let proof ← mkEqOfHEq proof
+    try
+      checkWithKernel proof
+    catch _ =>
+      return .rfl
+    let rhs   := thm.rhs.instantiateLevelParams thm.pattern.levelParams us
+    let rhs   ← share rhs
+    let expr  ← instantiateRevBetaS rhs args.toArray
+    if isSameExpr e expr then
+      return .rfl
+    else
+      return .step expr proof
+  else
+    return .rfl
+
 
 public def Theorems.rewrite (thms : Theorems) (d : Discharger := dischargeNone) : Simproc := fun e => do
   for (thm, numExtra) in thms.getMatchWithExtra e do
